theories/typing.v
@@ -112,12 +112,15 @@ Inductive Wt : context -> T -> tm -> tm -> Prop :=
   Γ ⊢ (tEq ℓ0 a b A) ; ℓ ∈ (tUniv i)
 
 (* Refactor the equality to include the grade for the term *)
-| T_J Γ t a b p A i j C ℓ ℓp ℓA ℓ0 ℓ1:
+| T_J Γ t a b p A i j C ℓ ℓp ℓT ℓ0 ℓ1:
   ℓp ⊆ ℓ ->
+  ℓ0 ⊆ ℓT ->
   Γ ⊢ a ; ℓ1 ∈ A ->
   Γ ⊢ b ; ℓ1 ∈ A ->
-  Γ ⊢ A ; ℓA ∈ (tUniv j) ->
+  Γ ⊢ A ; ℓT ∈ (tUniv j) ->
+  Γ ⊢ a ; ℓ0 ∈ A ->
   Γ ⊢ p ; ℓp ∈ (tEq ℓ0 a b A) ->
+  (* plug in a to show the admissibility lemma  *)
   ((ℓp, tEq ℓ0 (ren_tm shift a) (var_tm 0) (ren_tm shift A)) :: (ℓ1, A) :: Γ) ⊢ C ; ℓ0 ∈ (tUniv i) ->
   Γ ⊢ t ; ℓ ∈ (C [tRefl .: a ..]) ->
   Γ ⊢ (tJ C t p) ; ℓ ∈ (C [p .: b..])
